src/HOL/IMP/Abs_Int_Tests.thy
@@ -1,0 +1,68 @@
+theory Abs_Int_Tests
+imports ACom
+begin
+
+subsection "Test Programs"
+
+text{* For constant propagation: *}
+
+text{* Straight line code: *}
+definition "test1_const =
+ ''y'' ::= N 7;
+ ''z'' ::= Plus (V ''y'') (N 2);
+ ''y'' ::= Plus (V ''x'') (N 0)"
+
+text{* Conditional: *}
+definition "test2_const =
+ IF Less (N 41) (V ''x'') THEN ''x'' ::= N 5 ELSE ''x'' ::= N 5"
+
+text{* Conditional, test is relevant: *}
+definition "test3_const =
+ ''x'' ::= N 42;
+ IF Less (N 41) (V ''x'') THEN ''x'' ::= N 5 ELSE ''x'' ::= N 6"
+
+text{* While: *}
+definition "test4_const =
+ ''x'' ::= N 0; WHILE Bc True DO ''x'' ::= N 0"
+
+text{* While, test is relevant: *}
+definition "test5_const =
+ ''x'' ::= N 0; WHILE Less (V ''x'') (N 1) DO ''x'' ::= N 1"
+
+text{* Iteration is needed: *}
+definition "test6_const =
+  ''x'' ::= N 0; ''y'' ::= N 0; ''z'' ::= N 2;
+  WHILE Less (V ''x'') (N 1) DO (''x'' ::= V ''y''; ''y'' ::= V ''z'')"
+
+text{* For intervals: *}
+
+definition "test1_ivl =
+ ''y'' ::= N 7;
+ IF Less (V ''x'') (V ''y'')
+ THEN ''y'' ::= Plus (V ''y'') (V ''x'')
+ ELSE ''x'' ::= Plus (V ''x'') (V ''y'')"
+
+definition "test2_ivl =
+ WHILE Less (V ''x'') (N 100)
+ DO ''x'' ::= Plus (V ''x'') (N 1)"
+
+definition "test3_ivl =
+ ''x'' ::= N 7;
+ WHILE Less (V ''x'') (N 100)
+ DO ''x'' ::= Plus (V ''x'') (N 1)"
+
+definition "test4_ivl =
+ ''x'' ::= N 0; ''y'' ::= N 100; ''z'' ::= Plus (V ''x'') (V ''y'');
+ WHILE Less (V ''x'') (N 11)
+ DO (''x'' ::= Plus (V ''x'') (N 1); ''y'' ::= Plus (V ''y'') (N -1))"
+
+definition "test5_ivl =
+ ''x'' ::= N 0; ''y'' ::= N 0;
+ WHILE Less (V ''x'') (N 1000)
+ DO (''y'' ::= V ''x''; ''x'' ::= Plus (V ''x'') (N 1))"
+
+definition "test6_ivl =
+ ''x'' ::= N 0;
+ WHILE Less (V ''x'') (N 1) DO ''x'' ::= Plus (V ''x'') (N -1)"
+
+end
