src/HOL/IMP/Collecting.thy
@@ -1,0 +1,180 @@
+theory Collecting
+imports Complete_Lattice_ix ACom
+begin
+
+subsection "Collecting Semantics of Commands"
+
+subsubsection "Annotated commands as a complete lattice"
+
+(* Orderings could also be lifted generically (thus subsuming the
+instantiation for preord and order), but then less_eq_acom would need to
+become a definition, eg less_eq_acom = lift2 less_eq, and then proofs would
+need to unfold this defn first. *)
+
+instantiation acom :: (order) order
+begin
+
+fun less_eq_acom :: "('a::order)acom \<Rightarrow> 'a acom \<Rightarrow> bool" where
+"less_eq_acom (SKIP {S}) (SKIP {S'}) = (S \<le> S')" |
+"less_eq_acom (x ::= e {S}) (x' ::= e' {S'}) = (x=x' \<and> e=e' \<and> S \<le> S')" |
+"less_eq_acom (c1;c2) (c1';c2') = (less_eq_acom c1 c1' \<and> less_eq_acom c2 c2')" |
+"less_eq_acom (IF b THEN c1 ELSE c2 {S}) (IF b' THEN c1' ELSE c2' {S'}) =
+  (b=b' \<and> less_eq_acom c1 c1' \<and> less_eq_acom c2 c2' \<and> S \<le> S')" |
+"less_eq_acom ({Inv} WHILE b DO c {P}) ({Inv'} WHILE b' DO c' {P'}) =
+  (b=b' \<and> less_eq_acom c c' \<and> Inv \<le> Inv' \<and> P \<le> P')" |
+"less_eq_acom _ _ = False"
+
+lemma SKIP_le: "SKIP {S} \<le> c \<longleftrightarrow> (\<exists>S'. c = SKIP {S'} \<and> S \<le> S')"
+by (cases c) auto
+
+lemma Assign_le: "x ::= e {S} \<le> c \<longleftrightarrow> (\<exists>S'. c = x ::= e {S'} \<and> S \<le> S')"
+by (cases c) auto
+
+lemma Semi_le: "c1;c2 \<le> c \<longleftrightarrow> (\<exists>c1' c2'. c = c1';c2' \<and> c1 \<le> c1' \<and> c2 \<le> c2')"
+by (cases c) auto
+
+lemma If_le: "IF b THEN c1 ELSE c2 {S} \<le> c \<longleftrightarrow>
+  (\<exists>c1' c2' S'. c= IF b THEN c1' ELSE c2' {S'} \<and> c1 \<le> c1' \<and> c2 \<le> c2' \<and> S \<le> S')"
+by (cases c) auto
+
+lemma While_le: "{Inv} WHILE b DO c {P} \<le> w \<longleftrightarrow>
+  (\<exists>Inv' c' P'. w = {Inv'} WHILE b DO c' {P'} \<and> c \<le> c' \<and> Inv \<le> Inv' \<and> P \<le> P')"
+by (cases w) auto
+
+definition less_acom :: "'a acom \<Rightarrow> 'a acom \<Rightarrow> bool" where
+"less_acom x y = (x \<le> y \<and> \<not> y \<le> x)"
+
+instance
+proof
+  case goal1 show ?case by(simp add: less_acom_def)
+next
+  case goal2 thus ?case by (induct x) auto
+next
+  case goal3 thus ?case
+  apply(induct x y arbitrary: z rule: less_eq_acom.induct)
+  apply (auto intro: le_trans simp: SKIP_le Assign_le Semi_le If_le While_le)
+  done
+next
+  case goal4 thus ?case
+  apply(induct x y rule: less_eq_acom.induct)
+  apply (auto intro: le_antisym)
+  done
+qed
+
+end
+
+fun lift :: "('a set set \<Rightarrow> 'a set) \<Rightarrow> com \<Rightarrow> 'a set acom set \<Rightarrow> 'a set acom"
+where
+"lift F com.SKIP M = (SKIP {F {P. SKIP {P} : M}})" |
+"lift F (x ::= a) M = (x ::= a {F {P. x::=a {P} : M}})" |
+"lift F (c1;c2) M =
+  (lift F c1 {c1. \<exists>c2. c1;c2 : M}); (lift F c2 {c2. \<exists>c1. c1;c2 : M})" |
+"lift F (IF b THEN c1 ELSE c2) M =
+  IF b THEN lift F c1 {c1. \<exists>c2 P. IF b THEN c1 ELSE c2 {P} : M}
+       ELSE lift F c2 {c2. \<exists>c1 P. IF b THEN c1 ELSE c2 {P} : M}
+  {F {P. \<exists>c1 c2. IF b THEN c1 ELSE c2 {P} : M}}" |
+"lift F (WHILE b DO c) M =
+ {F {I. \<exists>c P. {I} WHILE b DO c {P} : M}}
+ WHILE b DO lift F c {c. \<exists>I P. {I} WHILE b DO c {P} : M}
+ {F {P. \<exists>I c. {I} WHILE b DO c {P} : M}}"
+
+interpretation Complete_Lattice_ix strip "lift Inter"
+proof
+  case goal1
+  have "a:A \<Longrightarrow> lift Inter (strip a) A \<le> a"
+  proof(induction a arbitrary: A)
+    case Semi from Semi.prems show ?case by(fastforce intro!: Semi.IH)
+  next
+    case If from If.prems show ?case by(fastforce intro!: If.IH)
+  next
+    case While from While.prems show ?case by(fastforce intro!: While.IH)
+  qed auto
+  with goal1 show ?case by auto
+next
+  case goal2
+  thus ?case
+  proof(induction b arbitrary: i A)
+    case Semi from Semi.prems show ?case by (fastforce intro!: Semi.IH)
+  next
+    case If from If.prems show ?case by (fastforce intro!: If.IH)
+  next
+    case While from While.prems show ?case by(fastforce intro: While.IH)
+  qed fastforce+
+next
+  case goal3
+  thus ?case
+  proof(induction i arbitrary: A)
+    case Semi from Semi.prems show ?case by (fastforce intro!: Semi.IH)
+  next
+    case If from If.prems show ?case by (fastforce intro!: If.IH)
+  next
+    case While from While.prems show ?case by(fastforce intro: While.IH)
+  qed auto
+qed
+
+lemma le_post: "c \<le> d \<Longrightarrow> post c \<le> post d"
+by(induction c d rule: less_eq_acom.induct) auto
+
+lemma le_strip: "c \<le> d \<Longrightarrow> strip c = strip d"
+by(induction c d rule: less_eq_acom.induct) auto
+
+lemma le_SKIP_iff: "c \<le> SKIP {P'} \<longleftrightarrow> (EX P. c = SKIP {P} \<and> P \<le> P')"
+by (cases c) simp_all
+
+lemma le_Assign_iff: "c \<le> x::=e {P'} \<longleftrightarrow> (EX P. c = x::=e {P} \<and> P \<le> P')"
+by (cases c) simp_all
+
+lemma le_Semi_iff: "c \<le> d1;d2 \<longleftrightarrow> (EX c1 c2. c = c1;c2 \<and> c1 \<le> d1 \<and> c2 \<le> d2)"
+by (cases c) simp_all
+
+lemma le_If_iff: "c \<le> IF b THEN d1 ELSE d2 {P'} \<longleftrightarrow>
+  (EX c1 c2 P. c = IF b THEN c1 ELSE c2 {P} \<and> c1 \<le> d1 \<and> c2 \<le> d2 \<and> P \<le> P')"
+by (cases c) simp_all
+
+lemma le_While_iff: "c \<le> {I'} WHILE b DO d {P'} \<longleftrightarrow>
+  (EX I c' P. c = {I} WHILE b DO c' {P} \<and> I \<le> I' \<and> c' \<le> d \<and> P \<le> P')"
+by (cases c) auto
+
+
+subsubsection "Collecting semantics"
+
+fun step_cs :: "state set \<Rightarrow> state set acom \<Rightarrow> state set acom" where
+"step_cs S (SKIP {P}) = (SKIP {S})" |
+"step_cs S (x ::= e {P}) =
+  (x ::= e {{s'. EX s:S. s' = s(x := aval e s)}})" |
+"step_cs S (c1; c2) = step_cs S c1; step_cs (post c1) c2" |
+"step_cs S (IF b THEN c1 ELSE c2 {P}) =
+   IF b THEN step_cs {s:S. bval b s} c1 ELSE step_cs {s:S. \<not> bval b s} c2
+   {post c1 \<union> post c2}" |
+"step_cs S ({Inv} WHILE b DO c {P}) =
+  {S \<union> post c} WHILE b DO (step_cs {s:Inv. bval b s} c) {{s:Inv. \<not> bval b s}}"
+
+definition CS :: "state set \<Rightarrow> com \<Rightarrow> state set acom" where
+"CS S c = lfp c (step_cs S)"
+
+lemma mono_step_cs_aux: "x \<le> y \<Longrightarrow> S \<subseteq> T \<Longrightarrow> step_cs S x \<le> step_cs T y"
+proof(induction x y arbitrary: S T rule: less_eq_acom.induct)
+  case 2 thus ?case by fastforce
+next
+  case 3 thus ?case by(simp add: le_post)
+next
+  case 4 thus ?case by(simp add: subset_iff)(metis le_post set_mp)+
+next
+  case 5 thus ?case by(simp add: subset_iff) (metis le_post set_mp)
+qed auto
+
+lemma mono_step_cs: "mono (step_cs S)"
+by(blast intro: monoI mono_step_cs_aux)
+
+lemma strip_step_cs: "strip(step_cs S c) = strip c"
+by (induction c arbitrary: S) auto
+
+lemmas lfp_cs_unfold = lfp_unfold[OF strip_step_cs mono_step_cs]
+
+lemma CS_unfold: "CS S c = step_cs S (CS S c)"
+by (metis CS_def lfp_cs_unfold)
+
+lemma strip_CS[simp]: "strip(CS S c) = c"
+by(simp add: CS_def)
+
+end
