src/HOL/IMP/Complete_Lattice_ix.thy
@@ -1,0 +1,55 @@
+theory Complete_Lattice_ix
+imports Main
+begin
+
+text{* A complete lattice is an ordered type where every set of elements has
+a greatest lower (and thus also a leats upper) bound. Sets are the
+prototypical complete lattice where the greatest lower bound is
+intersection. Sometimes that set of all elements of a type is not a complete
+lattice although all elements of the same shape form a complete lattice, for
+example lists of the same length, where the list elements come from a
+complete lattice. We will have exactly this situation with annotated
+commands. This theory introduces a slightly generalised version of complete
+lattices where elements have an ``index'' and only the set of elements with
+the same index form a complete lattice; the type as a whole is a disjoint
+union of complete lattices. Because sets are not types, this requires a
+special treatment. *}
+
+locale Complete_Lattice_ix =
+fixes ix :: "'a::order \<Rightarrow> 'i"
+and Glb :: "'i \<Rightarrow> 'a set \<Rightarrow> 'a"
+assumes Glb_lower: "\<forall>a\<in>A. ix a = i \<Longrightarrow> a \<in> A \<Longrightarrow> (Glb i A) \<le> a"
+and Glb_greatest: "\<forall>a\<in>A. b \<le> a \<Longrightarrow> ix b = i \<Longrightarrow> b \<le> (Glb i A)"
+and ix_Glb: "\<forall>a\<in>A. ix a = i \<Longrightarrow> ix(Glb i A) = i"
+begin
+
+definition lfp :: "'i \<Rightarrow> ('a \<Rightarrow> 'a) \<Rightarrow> 'a" where
+"lfp i f = Glb i {a. ix a = i \<and> f a \<le> a}"
+
+lemma index_lfp[simp]: "ix(lfp i f) = i"
+by(simp add: lfp_def ix_Glb)
+
+lemma lfp_lowerbound:
+  "\<lbrakk> ix a = i;  f a \<le> a \<rbrakk> \<Longrightarrow> lfp i f \<le> a"
+by (auto simp add: lfp_def intro: Glb_lower)
+
+lemma lfp_greatest:
+  "\<lbrakk> ix a = i;  \<And>u. \<lbrakk>ix u = i; f u \<le> u\<rbrakk> \<Longrightarrow> a \<le> u \<rbrakk> \<Longrightarrow> a \<le> lfp i f"
+by (auto simp add: lfp_def intro: Glb_greatest)
+
+lemma lfp_unfold: assumes "\<And>x. ix(f x) = ix x"
+and mono: "mono f" shows "lfp i f = f (lfp i f)"
+proof-
+  note assms(1)[simp]
+  have 1: "f (lfp i f) \<le> lfp i f"
+    apply(rule lfp_greatest)
+    apply(simp)
+    by (blast intro: lfp_lowerbound monoD[OF mono] order_trans)
+  have "lfp i f \<le> f (lfp i f)"
+    by (fastforce intro: 1 monoD[OF mono] lfp_lowerbound)
+  with 1 show ?thesis by(blast intro: order_antisym)
+qed
+
+end
+
+end
